Steel.Repr: use FList
We use flist (i.e. `(i : Fin.fin n) -> t i`) instead of dlist to represent
lists of selectors

experiment/Experiment.Steel.Repr.Fun.fst
@@ -3,6 +3,7 @@ module Experiment.Steel.Repr.Fun
 module U   = Learn.Util
 module L   = FStar.List.Pure
 module Ll  = Learn.List
+module Fl  = Learn.FList
 module Dl  = Learn.DList
 module ST  = Experiment.Steel.Repr.ST
 module Fin = FStar.Fin 
@@ -10,8 +11,8 @@ module Fin = FStar.Fin
 open Experiment.Steel.Repr.ST
 
 
-type post_t (a : Type) = a -> Dl.ty_list
-type post_v (#a : Type) (post : post_t a) (x : a) = Dl.dlist (post x)
+type post_t (a : Type) = a -> Fl.ty_list
+type post_v (#a : Type) (post : post_t a) (x : a) = Fl.flist (post x)
 type req_t = prop
 type ens_t (a : Type) (post : post_t a) = (x : a) -> post_v post x -> prop
 
@@ -20,7 +21,7 @@ type prog_tree : (a : Type u#a) -> (post : post_t u#a u#b a) -> Type u#(1 + max 
   | Tspec : (a : Type u#a) -> (post : post_t a) ->
             (req : req_t) -> (ens : ens_t a post) ->
             prog_tree a post
-  | Tret   : (a : Type u#a) -> (x : a) -> (post : post_t a) -> (sl : post_v post x) ->
+  | Tret   : (a : Type u#a) -> (x : a) -> (post : post_t a) -> (sl : Dl.dlist (post x)) ->
              prog_tree a post
   | Tbind  : (a : Type u#a) -> (b : Type u#a) ->
              (itm : post_t a) -> (post : post_t b) ->
@@ -50,7 +51,7 @@ and tree_ens (#a : Type) (#post : post_t a) (t : prog_tree a post)
   | Tspec _ _  _ ens ->
              ens
   | Tret _ x  post0 sl ->
-             (fun x' (sl' : post_v post x') -> x' == x /\ sl' == sl)
+             (fun x' (sl' : post_v post x') -> x' == x /\ sl' == Fl.flist_of_d sl)
   | Tbind a _  itm post0  f g ->
              (fun y (sl2 : post_v post y) ->
                (exists (x : a) (sl1 : post_v itm x) .
@@ -175,62 +176,63 @@ let post_Fun_of_ST
 let sel_Fun_of_ST
       (#a : Type u#a) (post : ST.post_t u#a u#b a)
       (#pre_n #post_n : nat) (s : ST.shape_tree pre_n post_n {post_has_len post post_n})
-      (x : a) (post_val : Dl.dlist (post x))
+      (x : a) (post_val : Fl.flist (post x))
   : post_v (post_Fun_of_ST post s) x
   = let p' = post_bij s in
-    Dl.initi 0 p'.post'_n _ (fun i -> Dl.index post_val (p'.post'_g i))
+    Fl.mk_flist (post_Fun_of_ST post s x)
+                (fun i -> U.cast (L.index (post_Fun_of_ST post s x) i) (post_val (p'.post'_g i)))
 
 unfold
 let return_Fun_post'_of_ST
       (#a : Type u#a) (post : ST.post_t u#a u#b a)
       (#pre_n #post_n : nat) (s : ST.shape_tree pre_n post_n {post_has_len post post_n})
-      (x : a) (post_val : Dl.dlist (post x))
+      (x : a) (post_val : Fl.flist (post x))
   : prog_tree a (post_Fun_of_ST post s)
-  = Tret a x (post_Fun_of_ST post s) (sel_Fun_of_ST post s x post_val)
+  = Tret a x (post_Fun_of_ST post s) (Fl.dlist_of_f (sel_Fun_of_ST post s x post_val))
 
 // TODO? remove the dependency in [t]
 let sel_ST_of_Fun
       (#a : Type) (#pre : ST.pre_t) (#post : ST.post_t a) (t : ST.prog_tree a pre post)
       (s : ST.prog_shape t)
-      (sl0 : Dl.dlist pre) (x : a) (sl1' : post_v (post_Fun_of_ST post s.shp) x)
-  : Dl.dlist (post x)
+      (sl0 : Fl.flist pre) (x : a) (sl1' : post_v (post_Fun_of_ST post s.shp) x)
+  : Fl.flist (post x)
   =
     let p' = post_bij s.shp in
-    Dl.initi_ty (post x)
+    Fl.mk_flist (post x)
              (fun i -> match post_src_of_shape s.shp i with
                     | Some j -> (**) post_src_ty t s x i;
                                U.cast (L.index (post x) i)
-                                      (Dl.index sl0 j)
+                                      (sl0 j)
                     | None   -> U.cast (L.index (post x) i)
-                                      (Dl.index sl1' (p'.post'_f i)))
+                                      (sl1' (p'.post'_f i)))
 
 #push-options "--z3rlimit 20"
 let sel_Fun_ST_Fun
       (#a : Type) (#pre : ST.pre_t) (#post : ST.post_t a) (t : ST.prog_tree a pre post)
       (s : ST.prog_shape t)
-      (sl0 : Dl.dlist pre) (x : a) (sl1' : post_v (post_Fun_of_ST post s.shp) x)
+      (sl0 : Fl.flist pre) (x : a) (sl1' : post_v (post_Fun_of_ST post s.shp) x)
   : Lemma (sel_Fun_of_ST post s.shp x (sel_ST_of_Fun t s sl0 x sl1') == sl1')
-  = Dl.dlist_extensionality
+  = Fl.flist_extensionality
          (sel_Fun_of_ST post s.shp x (sel_ST_of_Fun t s sl0 x sl1')) sl1'
     begin fun i ->
       let p' = post_bij s.shp in
       let post_ST = sel_ST_of_Fun t s sl0 x sl1' in
       calc (==) {
-        Dl.index (sel_Fun_of_ST post s.shp x post_ST) i;
-      == {}
+        sel_Fun_of_ST post s.shp x post_ST i;
+      == { (*_ by T.(trefl ())*) }// FIXME: interactive mode fails here when loading without a .checked
         U.cast (L.index (post_Fun_of_ST post s.shp x) i)
-          (Dl.index post_ST ((post_bij s.shp).post'_g i));
+          (post_ST ((post_bij s.shp).post'_g i));
       == {}
-        Dl.index sl1' ((post_bij s.shp).post'_f ((post_bij s.shp).post'_g i));
+        sl1' ((post_bij s.shp).post'_f ((post_bij s.shp).post'_g i));
       == {}
-        Dl.index sl1' i;
+        sl1' i;
       }
    end
 #pop-options
 
 
 let post_Fun_of_ST__frame
-      (#a : Type) (post : ST.post_t a) (frame: Dl.ty_list)
+      (#a : Type) (post : ST.post_t a) (frame: Fl.ty_list)
       (pre_n : nat) (post_n : nat {post_has_len post post_n}) (f : shape_tree pre_n post_n)
   : Lemma (ensures post_Fun_of_ST (ST.frame_post post frame) (Sframe pre_n post_n (L.length frame) f)
                 == post_Fun_of_ST post f)
@@ -269,10 +271,10 @@ let post_Fun_of_ST__ret
 let rec repr_Fun_of_ST
           (#a : Type u#a) (#pre : ST.pre_t u#b) (#post : ST.post_t u#a u#b a)
           (t : ST.prog_tree a pre post)
-  : Tot ((s : ST.prog_shape t) -> Dl.dlist pre -> prog_tree a (post_Fun_of_ST post s.shp))
+  : Tot ((s : ST.prog_shape t) -> Fl.flist pre -> prog_tree a (post_Fun_of_ST post s.shp))
         (decreases t)
   = match t as t'
-      returns (s : ST.prog_shape t) -> Dl.dlist pre ->
+      returns (s : ST.prog_shape t) -> Fl.flist pre ->
               prog_tree a (post_Fun_of_ST post s.shp)
     with
     | ST.Tequiv pre post0 p -> fun s sl0 ->
@@ -280,7 +282,7 @@ let rec repr_Fun_of_ST
     | ST.Tframe a pre post frame f -> fun s sl0 ->
             (**) let Sframe _ post_n _ shp_f = s.shp in
             (**) post_Fun_of_ST__frame post frame (L.length pre) post_n shp_f;
-            let sl0' : Dl.dlist pre = (Dl.splitAt_ty pre frame sl0)._1 in
+            let sl0' : Fl.flist pre = (Fl.splitAt_ty pre frame sl0)._1 in
             repr_Fun_of_ST f (ST.mk_prog_shape f shp_f) sl0'
     | ST.Tspec a pre post req ens -> fun s sl0 ->
             (**) let Sspec _ post_n = s.shp in
@@ -289,7 +291,7 @@ let rec repr_Fun_of_ST
     | ST.Tret a x post -> fun s sl ->
             (**) let Sret post_n = s.shp in
             (**) post_Fun_of_ST__ret post post_n;
-            Tret a x (U.eta post) sl
+            Tret a x (U.eta post) (Fl.dlist_of_f sl)
     | ST.Tbind a b pre itm post f g -> fun s sl0 ->
             (**) let Sbind _ itm_n post_n shp_f shp_g = s.shp in
             (**) let s_f = ST.mk_prog_shape f shp_f in
@@ -308,7 +310,7 @@ let rec repr_Fun_of_ST
                        (repr_Fun_of_ST (g x) s_g sl0) (fun y sl1' ->
             let sl1 = sel_ST_of_Fun (g x) s_g sl0 y sl1' in
             return_Fun_post'_of_ST post s.shp y sl1))
-    
+
 #pop-options
 
 
@@ -316,39 +318,39 @@ let rec repr_Fun_of_ST
 
 #push-options "--fuel 1 --ifuel 0"
 
-let post_eq_src (#pre #post : Dl.ty_list) (sl0 : Dl.dlist pre) (sl1 : Dl.dlist post)
+let post_eq_src (#pre #post : Fl.ty_list) (sl0 : Fl.flist pre) (sl1 : Fl.flist post)
                 (s : post_src (L.length pre) (L.length post))
   : prop
   = forall (i : Fin.fin (L.length post)) .
-      Some? (s i) ==> Dl.index sl1 i === Dl.index sl0 (Some?.v (s i))
+      Some? (s i) ==> sl1 i === sl0 (Some?.v (s i))
 
 let sel_ST_of_Fun_eq_src
       #a #pre #post (t : ST.prog_tree a pre post) (s : ST.prog_shape t)
-      (sl0 : Dl.dlist pre) (x : a) (sl1' : post_v (post_Fun_of_ST post s.shp) x)
+      (sl0 : Fl.flist pre) (x : a) (sl1' : post_v (post_Fun_of_ST post s.shp) x)
   : Lemma (post_eq_src sl0 (sel_ST_of_Fun t s sl0 x sl1') (post_src_of_shape s.shp))
   = introduce forall (i : Fin.fin s.post_len) .
       Some? (post_src_of_shape s.shp i) ==>
-      Dl.index (sel_ST_of_Fun t s sl0 x sl1') i === Dl.index sl0 (Some?.v (post_src_of_shape s.shp i))
+      sel_ST_of_Fun t s sl0 x sl1' i === sl0 (Some?.v (post_src_of_shape s.shp i))
     with introduce _ ==> _
     with _ . post_src_ty t s x i
 
 #push-options "--z3rlimit 20"
 let post_eq_src_ST_Fun_ST
       #a #pre #post  (t : ST.prog_tree a pre post) (s : ST.prog_shape t)
-      (sl0 : Dl.dlist pre) (x : a) (sl1 : Dl.dlist (post x))
+      (sl0 : Fl.flist pre) (x : a) (sl1 : Fl.flist (post x))
   : Lemma (requires post_eq_src sl0 sl1 (post_src_of_shape s.shp))
           (ensures  sel_ST_of_Fun t s sl0 x (sel_Fun_of_ST post s.shp x sl1) == sl1)
   =
-    Dl.dlist_extensionality (sel_ST_of_Fun t s sl0 x (sel_Fun_of_ST post s.shp x sl1)) sl1
+    Fl.flist_extensionality (sel_ST_of_Fun t s sl0 x (sel_Fun_of_ST post s.shp x sl1)) sl1
     begin fun i ->
       match post_src_of_shape s.shp i with
       | Some j -> post_src_ty t s x i;
                  calc (==) {
-                   Dl.index (sel_ST_of_Fun t s sl0 x (sel_Fun_of_ST post s.shp x sl1)) i;
+                   sel_ST_of_Fun t s sl0 x (sel_Fun_of_ST post s.shp x sl1) i;
                  == {}
-                   U.cast (L.index (post x) i) (Dl.index sl0 j);
+                   U.cast (L.index (post x) i) (sl0 j);
                  == {(*by [post_eq_src] *)}
-                   Dl.index sl1 i;
+                   sl1 i;
                  }
       | None -> ()
     end
@@ -357,7 +359,7 @@ let post_eq_src_ST_Fun_ST
 (* TODO? def de post_eq_src *)
 let post_eq_src_iff
       #a #pre #post (t : ST.prog_tree a pre post) (s : ST.prog_shape t)
-      (sl0 : Dl.dlist pre) (x : a) (sl1 : Dl.dlist (post x))
+      (sl0 : Fl.flist pre) (x : a) (sl1 : Fl.flist (post x))
   : Lemma (post_eq_src sl0 sl1 (post_src_of_shape s.shp)
            <==> sl1 == sel_ST_of_Fun t s sl0 x (sel_Fun_of_ST post s.shp x sl1))
   = sel_ST_of_Fun_eq_src t s sl0 x (sel_Fun_of_ST post s.shp x sl1);
@@ -366,20 +368,20 @@ let post_eq_src_iff
 
 unfold
 let req_equiv #a #pre #post (t : ST.prog_tree a pre post) (s : ST.prog_shape t)
-      (sl0 : Dl.dlist pre)
+      (sl0 : Fl.flist pre)
   : prop
   = ST.tree_req t sl0 <==> tree_req (repr_Fun_of_ST t s sl0)
 
 unfold
 let ens_equiv #a #pre #post (t : ST.prog_tree a pre post) (s : ST.prog_shape t)
-      (sl0 : Dl.dlist pre) (res : a) (sl1 : Dl.dlist (post res))
+      (sl0 : Fl.flist pre) (res : a) (sl1 : Fl.flist (post res))
   : prop
   = ST.tree_ens t sl0 res sl1 <==>
    (post_eq_src sl0 sl1 (post_src_of_shape s.shp) /\
     tree_ens (repr_Fun_of_ST t s sl0) res (sel_Fun_of_ST post s.shp res sl1))
 
 let ens_equiv_rev #a #pre #post (t : ST.prog_tree a pre post) (s : ST.prog_shape t)
-      (sl0 : Dl.dlist pre) (res : a) (sl1' : post_v (post_Fun_of_ST post s.shp) res)
+      (sl0 : Fl.flist pre) (res : a) (sl1' : post_v (post_Fun_of_ST post s.shp) res)
   : Lemma (requires ens_equiv t s sl0 res (sel_ST_of_Fun t s sl0 res sl1'))
           (ensures  ST.tree_ens t sl0 res (sel_ST_of_Fun t s sl0 res sl1') <==>
                     tree_ens (repr_Fun_of_ST t s sl0) res sl1')
@@ -392,7 +394,7 @@ let repr_Fun_of_ST_ens__Tframe a pre post frame f
       (post_n : nat {ST.post_has_len post post_n})
       (shp_f : ST.shape_tree _ post_n {ST.prog_has_shape f shp_f})
       sl0 x sl1
-      (ens_eq_f : (sl0' : Dl.dlist pre) -> (sl1' : Dl.dlist (post x)) ->
+      (ens_eq_f : (sl0' : Fl.flist pre) -> (sl1' : Fl.flist (post x)) ->
                   Lemma (ens_equiv f (ST.mk_prog_shape f shp_f) sl0' x sl1'))
   : Lemma (ensures ens_equiv (ST.Tframe a pre post frame f)
                              (ST.mk_prog_shape _ (Sframe _ _ (L.length frame) shp_f)) sl0 x sl1)
@@ -405,8 +407,8 @@ let repr_Fun_of_ST_ens__Tframe a pre post frame f
     let post_Fun  = sel_Fun_of_ST (ST.frame_post post frame) s.shp x sl1             in
 
     assert (ens_equiv t s sl0 x sl1 == (
-     (let sl0', frame0 = Dl.splitAt_ty pre      frame sl0 in
-      let sl1', frame1 = Dl.splitAt_ty (post x) frame sl1 in
+     (let sl0', frame0 = Fl.splitAt_ty pre      frame sl0 in
+      let sl1', frame1 = Fl.splitAt_ty (post x) frame sl1 in
       frame1 == frame0 /\ ST.tree_ens f sl0' x sl1')
     <==>
       (post_eq_src sl0 sl1 (post_src_of_shape s.shp) /\
@@ -414,50 +416,56 @@ let repr_Fun_of_ST_ens__Tframe a pre post frame f
     )) by T.(trefl ());
 
     assert (repr_Fun_of_ST t s sl0 == (
-      repr_Fun_of_ST f s_f (Dl.splitAt_ty pre frame sl0)._1
+      repr_Fun_of_ST f s_f (Fl.splitAt_ty pre frame sl0)._1
     )) by T.(trefl ());
     
-    let sl0', frame0 = Dl.splitAt_ty pre      frame sl0 in
-    let sl1', frame1 = Dl.splitAt_ty (post x) frame sl1 in
+    let sl0', frame0 = Fl.splitAt_ty pre      frame sl0 in
+    let sl1', frame1 = Fl.splitAt_ty (post x) frame sl1 in
     let post_Fun' = sel_Fun_of_ST post shp_f x sl1'     in
     let post_src   = post_src_of_shape s.shp            in
     let post_src_f = post_src_of_shape shp_f            in
     let bij = post_bij shp_f                            in
 
     ens_eq_f sl0' sl1';
-    Dl.splitAt_ty_append pre frame sl0;
-    Dl.splitAt_ty_append (post x) frame sl1;
-    Dl.dlist_extensionality post_Fun post_Fun'
-      (fun i -> Dl.append_index sl1' frame1 (bij.post'_g i));
+    Fl.flist_extensionality post_Fun post_Fun' (fun i -> ());
 
     let eq0 : prop = frame1 == frame0 /\ post_eq_src sl0' sl1' post_src_f in
     let eq1 : prop = post_eq_src sl0 sl1 post_src                         in
-    introduce eq0 ==> eq1 with _ .
+    introduce (eq0 ==> eq1) /\ (eq1 ==> eq0)
+    with introduce eq0 ==> eq1 with _ .
+      let hyp (i : Fin.fin post_n {Some? (post_src_f i)})
+        : Lemma (sl1' i === sl0' (Some?.v (post_src_f i))) = ()
+      in
       introduce forall (i : Fin.fin (post_n + L.length frame) {Some? (post_src i)}) .
-                  Dl.index sl1 i === Dl.index sl0 (Some?.v (post_src i))
+                  sl1 i === sl0 (Some?.v (post_src i))
       with begin
-        Dl.append_index sl1' frame1 i;
+        Fl.append_index sl1' frame1 i;
         if i < post_n
-        then Dl.append_index sl0' frame0 (Some?.v (post_src_f i))
-        else Dl.append_index sl0' frame0 (i - post_n + L.length pre)
-      end;
-    introduce eq1 ==> eq0
-      with _ .
+        then begin
+          hyp i;
+          Fl.append_index sl0' frame0 (Some?.v (post_src_f i))
+        end else begin
+          assert (sl1 i === frame1 (i - post_n));
+          Fl.append_index sl0' frame0 (i - post_n + L.length pre);
+          assert (sl0 (Some?.v (post_src i)) === frame0 (i - post_n))
+        end
+      end
+    and introduce eq1 ==> eq0 with _ .
       let hyp (i : Fin.fin (post_n + L.length frame) {Some? (post_src i)})
-        : Lemma (Dl.index sl1 i === Dl.index sl0 (Some?.v (post_src i))) = ()
+        : Lemma (sl1 i === sl0 (Some?.v (post_src i))) = ()
       in
       introduce frame1 == frame0 /\ post_eq_src sl0' sl1' post_src_f
-      with Dl.dlist_extensionality frame1 frame0 begin fun i ->
+      with Fl.flist_extensionality frame1 frame0 begin fun i ->
         hyp (i + post_n);
-        Dl.append_index sl1' frame1 (i + post_n);
-        Dl.append_index sl0' frame0 (i + L.length pre)
+        Fl.append_index sl1' frame1 (i + post_n);
+        Fl.append_index sl0' frame0 (i + L.length pre)
       end and
       introduce forall (i : Fin.fin post_n {Some? (post_src_f i)}) .
-                  Dl.index sl1' i === Dl.index sl0' (Some?.v (post_src_f i))
+                  sl1' i === sl0' (Some?.v (post_src_f i))
       with begin
         hyp i;
-        Dl.append_index sl1' frame1 i;
-        Dl.append_index sl0' frame0 (Some?.v (post_src_f i))
+        Fl.append_index sl1' frame1 i;
+        Fl.append_index sl0' frame0 (Some?.v (post_src_f i))
       end
 #pop-options
 
@@ -471,9 +479,9 @@ let repr_Fun_of_ST_req__Tbind a b pre (itm : ST.post_t a) post
       (shp_f : ST.shape_tree _     itm_n  {ST.prog_has_shape f shp_f})
       (shp_g : ST.shape_tree itm_n post_n {forall (x : a) . ST.prog_has_shape (g x) shp_g})
       sl0
-      (req_eq_g : (x : a) -> (sl1 : Dl.dlist (itm x)) ->
+      (req_eq_g : (x : a) -> (sl1 : Fl.flist (itm x)) ->
                   Lemma (req_equiv (g x) (ST.mk_prog_shape (g x) shp_g) sl1))
-      (ens_eq_f : (x : a) -> (sl1 : Dl.dlist (itm x)) ->
+      (ens_eq_f : (x : a) -> (sl1 : Fl.flist (itm x)) ->
                   Lemma (ens_equiv f (ST.mk_prog_shape f shp_f) sl0 x sl1))
   : Lemma
       (requires ST.tree_req f sl0 <==> tree_req (repr_Fun_of_ST f (ST.mk_prog_shape f shp_f) sl0))
@@ -485,12 +493,12 @@ let repr_Fun_of_ST_req__Tbind a b pre (itm : ST.post_t a) post
     let s_f = ST.mk_prog_shape f shp_f                                          in
     let s_g (x : a) = ST.mk_prog_shape (g x) shp_g                              in
     let r_f = repr_Fun_of_ST f s_f sl0                                          in
-    let r_g (x : a) (sl1 : Dl.dlist (itm x)) = repr_Fun_of_ST (g x) (s_g x) sl1 in
+    let r_g (x : a) (sl1 : Fl.flist (itm x)) = repr_Fun_of_ST (g x) (s_g x) sl1 in
     let itm' = post_Fun_of_ST itm s_f.shp                                       in
 
     assert (req_equiv t s sl0 == (
       (ST.tree_req f sl0 /\
-      (forall (x : a) (sl1 : Dl.dlist (itm x)) .
+      (forall (x : a) (sl1 : Fl.flist (itm x)) .
         ST.tree_ens f sl0 x sl1 ==> ST.tree_req (g x) sl1))
     <==>
       (tree_req r_f /\
@@ -503,13 +511,13 @@ let repr_Fun_of_ST_req__Tbind a b pre (itm : ST.post_t a) post
     )) by T.(trefl ());
 
     introduce forall (x : a) . ST.tree_req f sl0 ==> (
-      (forall (sl1 : Dl.dlist (itm x)) . ST.tree_ens f sl0 x sl1 ==> ST.tree_req (g x) sl1) <==>
+      (forall (sl1 : Fl.flist (itm x)) . ST.tree_ens f sl0 x sl1 ==> ST.tree_req (g x) sl1) <==>
       (forall (sl1' : post_v itm' x) .
         tree_ens r_f x sl1' ==>
         tree_req (r_g x (sel_ST_of_Fun f s_f sl0 x sl1'))))
       with introduce _ ==> _
       with _ . begin
-        introduce forall (sl1 : Dl.dlist (itm x)) . ens_equiv f s_f sl0 x sl1
+        introduce forall (sl1 : Fl.flist (itm x)) . ens_equiv f s_f sl0 x sl1
           with ens_eq_f x sl1;
         FStar.Classical.forall_intro (post_eq_src_iff f s_f sl0 x);
         forall_morph_iff #(post_v itm' x)
@@ -530,9 +538,9 @@ let repr_Fun_of_ST_ens__Tbind a b pre (itm : ST.post_t a) post
       (shp_f : ST.shape_tree _     itm_n  {ST.prog_has_shape f shp_f})
       (shp_g : ST.shape_tree itm_n post_n {forall (x : a) . ST.prog_has_shape (g x) shp_g})
       sl0 y sl2
-      (ens_eq_f : (x : a) -> (sl1 : Dl.dlist (itm x)) ->
+      (ens_eq_f : (x : a) -> (sl1 : Fl.flist (itm x)) ->
                   Lemma (ens_equiv f (ST.mk_prog_shape f shp_f) sl0 x sl1))
-      (ens_eq_g : (x : a) -> (sl1 : Dl.dlist (itm x)) ->
+      (ens_eq_g : (x : a) -> (sl1 : Fl.flist (itm x)) ->
                   Lemma (ens_equiv (g x) (ST.mk_prog_shape (g x) shp_g) sl1 y sl2))
   : Lemma
       (ensures  ens_equiv (ST.Tbind a b pre itm post f g)
@@ -543,14 +551,14 @@ let repr_Fun_of_ST_ens__Tbind a b pre (itm : ST.post_t a) post
     let s_f = ST.mk_prog_shape f shp_f                                          in
     let s_g (x : a) = ST.mk_prog_shape (g x) shp_g                              in
     let r_f = repr_Fun_of_ST f s_f sl0                                          in
-    let r_g (x : a) (sl1 : Dl.dlist (itm x)) = repr_Fun_of_ST (g x) (s_g x) sl1 in
+    let r_g (x : a) (sl1 : Fl.flist (itm x)) = repr_Fun_of_ST (g x) (s_g x) sl1 in
     let itm'  = post_Fun_of_ST itm s_f.shp                                      in
     let post'g = post_Fun_of_ST post shp_g                                      in
     let post'  = post_Fun_of_ST post s.shp                                      in
     let sl2' : post_v post' y = sel_Fun_of_ST post s.shp y sl2                  in
 
     assert (ens_equiv t s sl0 y sl2 ==
-      ((exists (x : a) (sl1 : Dl.dlist (itm x)) .
+      ((exists (x : a) (sl1 : Fl.flist (itm x)) .
          ST.tree_ens f sl0 x sl1 /\ ST.tree_ens (g x) sl1 y sl2)
      <==>
       (post_eq_src sl0 sl2 (post_src_of_shape s.shp) /\
@@ -560,15 +568,15 @@ let repr_Fun_of_ST_ens__Tbind a b pre (itm : ST.post_t a) post
         let r_g = r_g x sl1                      in
         (exists (yg : b) (sl2g : post_v (post_Fun_of_ST post #(L.length (itm x)) shp_g) yg) .
          tree_ens r_g yg sl2g /\
-        (let sl2f : Dl.dlist (post yg) = sel_ST_of_Fun (g x) (s_g x) sl1 yg sl2g in
-         tree_ens (Tret b yg post' (sel_Fun_of_ST post s.shp yg sl2f)) y sl2'
+        (let sl2f : Fl.flist (post yg) = sel_ST_of_Fun (g x) (s_g x) sl1 yg sl2g in
+         tree_ens (Tret b yg post' (Fl.dlist_of_f (sel_Fun_of_ST post s.shp yg sl2f))) y sl2'
          ))))))
     )) by T.(trefl ());
 
     assert (post_eq_src sl0 sl2 (post_src_of_shape s.shp));
 
     introduce forall (x : a) .
-       (exists (sl1 : Dl.dlist (itm x)) . ST.tree_ens f sl0 x sl1 /\ ST.tree_ens (g x) sl1 y sl2)
+       (exists (sl1 : Fl.flist (itm x)) . ST.tree_ens f sl0 x sl1 /\ ST.tree_ens (g x) sl1 y sl2)
     <==> (exists (sl1' : post_v itm' x) .
          tree_ens r_f x sl1' /\
        (let sl1 = sel_ST_of_Fun f s_f sl0 x sl1' in
@@ -578,7 +586,7 @@ let repr_Fun_of_ST_ens__Tbind a b pre (itm : ST.post_t a) post
          sl2' == sel_Fun_of_ST post s.shp y (sel_ST_of_Fun (g x) (s_g x) sl1 y sl2g)
          )))
     with begin
-      introduce forall (sl2g : post_v post'g y) (sl1 : Dl.dlist (itm x)) .
+      introduce forall (sl2g : post_v post'g y) (sl1 : Fl.flist (itm x)) .
         sl2' == sel_Fun_of_ST post s.shp y (sel_ST_of_Fun (g x) (s_g x) sl1 y sl2g)
         <==> (sl2g == sel_Fun_of_ST post shp_g y sl2 /\
            post_eq_src sl1 sl2 (post_src_of_shape shp_g))
@@ -641,7 +649,7 @@ let repr_Fun_of_ST_ens__TbindP a b pre post
       (exists (yg : b) (sl1g : post_v (post_Fun_of_ST post #(L.length #Type pre) shp_g) yg) .
        tree_ens (r_g x) yg sl1g /\
       (let sl1f = sel_ST_of_Fun (g x) (s_g x) sl0 yg sl1g in
-       y == yg /\ sl1' == sel_Fun_of_ST post s.shp yg sl1f
+       y == yg /\ sl1' == Fl.flist_of_d (Fl.dlist_of_f (sel_Fun_of_ST post s.shp yg sl1f))
       )))))
     )) by T.(trefl ());
 
@@ -674,22 +682,22 @@ let repr_Fun_of_ST_ens__TbindP a b pre post
 let rec repr_Fun_of_ST_req
   (#a : Type u#a) (#pre : ST.pre_t u#b) (#post : ST.post_t u#a u#b a)
   (t : ST.prog_tree a pre post) (s : ST.prog_shape t)
-  (sl0 : Dl.dlist pre)
+  (sl0 : Fl.flist pre)
   : Lemma (ensures req_equiv t s sl0) (decreases t)
   = ST.match_prog_tree t
-    (fun a pre post t -> (s : ST.prog_shape t) -> (sl0 : Dl.dlist pre) ->
+    (fun a pre post t -> (s : ST.prog_shape t) -> (sl0 : Fl.flist pre) ->
        squash (ST.tree_req t sl0 <==> tree_req (repr_Fun_of_ST t s sl0)))
     (fun (*ST.Tequiv*) pre post0 p -> fun s sl0 -> ())
     begin fun (*ST.Tframe*) a pre post frame f -> fun s sl0 ->
       let Sframe pre_n post_n frame_n shp_f = s.shp in 
-      let sl0' : Dl.dlist pre = (Dl.splitAt_ty pre frame sl0)._1 in
+      let sl0' : Fl.flist pre = (Fl.splitAt_ty pre frame sl0)._1 in
       repr_Fun_of_ST_req f (ST.mk_prog_shape f shp_f) sl0'
     end
     (fun (*ST.Tspec*) a pre post req ens -> fun s sl0 -> ())
     (fun (*ST.Tret*) a x post -> fun s sl0 -> ())
     begin fun (*ST.Tbind*) a b pre itm post f g -> fun s sl0 ->
-      let Sbind _ itm_n post_n shp_f shp_g = s.shp in
-      let s_f = ST.mk_prog_shape f shp_f in
+      let Sbind _ itm_n post_n shp_f shp_g = s.shp   in
+      let s_f = ST.mk_prog_shape f shp_f             in
       let s_g (x : a) = ST.mk_prog_shape (g x) shp_g in
       repr_Fun_of_ST_req f s_f sl0;
       repr_Fun_of_ST_req__Tbind a b pre itm post f g itm_n post_n shp_f shp_g sl0
@@ -697,9 +705,9 @@ let rec repr_Fun_of_ST_req
         (fun x sl1 -> repr_Fun_of_ST_ens f s_f sl0 x sl1)
     end
     begin fun (*ST.TbindP*) a b pre post wp f g -> fun s sl0 ->
-      let SbindP _ post_n shp_g = s.shp in
+      let SbindP _ post_n shp_g = s.shp              in
       let s_g (x : a) = ST.mk_prog_shape (g x) shp_g in
-      let pt0 x = ST.tree_req (g x) sl0 in
+      let pt0 x = ST.tree_req (g x) sl0              in
       let pt1 x = tree_req (repr_Fun_of_ST (g x) (s_g x) sl0) /\
                     (forall (y : b) (sl1' : post_v (post_Fun_of_ST post #(L.length #Type pre) shp_g) y) .
                     tree_ens (repr_Fun_of_ST (g x) (s_g x) sl0) y sl1' ==> True) in
@@ -724,17 +732,19 @@ let rec repr_Fun_of_ST_req
 and repr_Fun_of_ST_ens
   (#a : Type u#a) (#pre : ST.pre_t u#b) (#post : ST.post_t u#a u#b a)
   (t : ST.prog_tree a pre post) (s : ST.prog_shape t)
-  (sl0 : Dl.dlist pre) (res : a) (sl1 : Dl.dlist (post res))
+  (sl0 : Fl.flist pre) (res : a) (sl1 : Fl.flist (post res))
   : Lemma (ensures ens_equiv t s sl0 res sl1)
           (decreases t)
   = ST.match_prog_tree t
     (fun a pre post t -> (s : ST.prog_shape t) ->
-       (sl0 : Dl.dlist pre) -> (res : a) -> (sl1 : Dl.dlist (post res)) ->
+       (sl0 : Fl.flist pre) -> (res : a) -> (sl1 : Fl.flist (post res)) ->
        squash (ens_equiv t s sl0 res sl1))
     begin fun (*ST.Tequiv*) pre post0 p -> fun s sl0 U.Unit' sl1 ->
-      introduce (forall (i : Fin.fin (L.length post0)) . Dl.index sl1 i === Dl.index sl0 (p i)) ==>
-                sl1 == Dl.apply_perm_r p sl0
-        with _ . Dl.dlist_extensionality sl1 (Dl.apply_perm_r p sl0) (fun _ -> ())
+      introduce (forall (i : Fin.fin (L.length post0)) . sl1 i === sl0 (p i)) ==>
+                sl1 == Fl.apply_perm_r p sl0
+        with _ . Fl.flist_extensionality sl1 (Fl.apply_perm_r p sl0) (fun _ -> ());
+      Fl.nil_uniq (sel_Fun_of_ST (const_post post0) s.shp U.Unit' sl1);
+      Fl.nil_uniq (Fl.flist_of_d Dl.DNil)
     end
     begin fun (*ST.Tframe*) a pre post frame f -> fun s sl0 x sl1 ->
       let Sframe pre_n post_n frame_n shp_f = s.shp in 
@@ -744,23 +754,23 @@ and repr_Fun_of_ST_ens
     begin fun (*ST.Tspec*) a pre post req ens -> fun s sl0 x sl1 ->
       let Sspec pre_n post_n = s.shp in
       post_Fun_of_ST__spec post pre_n post_n;
-      Dl.dlist_extensionality (sel_Fun_of_ST post s.shp x sl1) sl1 (fun _ -> ())
+      Fl.flist_extensionality (sel_Fun_of_ST post s.shp x sl1) sl1 (fun _ -> ())
     end
     begin fun (*ST.Tret*) a x post -> fun s sl0 x sl1 ->
       let Sret post_n = s.shp in
       post_Fun_of_ST__ret post post_n;
-      Dl.dlist_extensionality (sel_Fun_of_ST post s.shp x sl1) sl1 (fun _ -> ())
+      Fl.flist_extensionality (sel_Fun_of_ST post s.shp x sl1) sl1 (fun _ -> ())
     end
     begin fun (*ST.Tbind*) a b pre itm post f g -> fun s sl0 y sl2 ->
-      let Sbind _ itm_n post_n shp_f shp_g = s.shp in
-      let s_f = ST.mk_prog_shape f shp_f in
+      let Sbind _ itm_n post_n shp_f shp_g = s.shp   in
+      let s_f = ST.mk_prog_shape f shp_f             in
       let s_g (x : a) = ST.mk_prog_shape (g x) shp_g in
       repr_Fun_of_ST_ens__Tbind a b pre itm post f g itm_n post_n shp_f shp_g sl0 y sl2
         (fun x sl1 -> repr_Fun_of_ST_ens f s_f sl0 x sl1)
         (fun x sl1 -> repr_Fun_of_ST_ens (g x) (s_g x) sl1 y sl2)
     end
     begin fun (*ST.TbindP*) a b pre post wp f g -> fun s sl0 y sl1 ->
-      let SbindP _ post_n shp_g = s.shp in
+      let SbindP _ post_n shp_g = s.shp              in
       let s_g (x : a) = ST.mk_prog_shape (g x) shp_g in
       repr_Fun_of_ST_ens__TbindP a b pre post wp f g post_n shp_g sl0 y sl1
         (fun x -> repr_Fun_of_ST_ens (g x) (s_g x) sl0 y sl1)
@@ -772,7 +782,6 @@ and repr_Fun_of_ST_ens
 
 (*** Steel.Repr.Fun --> Repr.Fun *)
 
-module Uv  = FStar.Universe
 module Fun = Experiment.Repr.Fun
 
 noeq
@@ -784,43 +793,13 @@ type sl_tys_t : Type u#(max a b + 1)= {
 noeq
 type sl_tys_v (ty : sl_tys_t u#a u#b) : Type u#(max a (b + 1)) = {
   val_v : ty.val_t;
-  sel_v : Dl.dlist (ty.sel_t val_v)
+  sel_v : Fl.flist (ty.sel_t val_v)
 }
-
-
-let partial_app_dlist (src0 : Type u#s) (src : Dl.ty_list u#s) (dst : Type u#d) (f : Dl.dlist (src0 :: src) -> dst)
-                      (x : src0) (xs : Dl.dlist src) : dst
-  = f Dl.(DCons src0 x src xs)
-
-/// One could define [forall_dlist] with type:
-///   [Pure Type0 (requires True) (ensures fun p -> p <==> (forall (xs : Dl.dlist ty) . f xs))]
-/// However, the refinement on the result is keept during normalization and yields terms that cannot reduce fully.
-/// For this reason, [forall_dlist] is defined with type [Type0] and we prove separately a lemma (with a pattern)
-/// to use equivalence during proofs.
-/// The same holds for [sl_all], [exists_dlist] and [sl_ex].
-
-let rec forall_dlist (ty : Dl.ty_list) (f : Dl.dlist ty -> Type0)
-  : Tot Type0 (decreases ty)
-  = match ty with
-  | []      -> f Dl.DNil
-  | t0 :: ts -> (forall (x : t0) . forall_dlist ts (partial_app_dlist t0 ts Type0 f x))
-
-let rec forall_dlist_iff (ty : Dl.ty_list) (f : Dl.dlist ty -> Type0)
-  : Lemma (ensures forall_dlist ty f <==> (forall (xs : Dl.dlist ty) . f xs)) (decreases ty)
-          [SMTPat (forall_dlist ty f)]
-  = match ty with
-  | [] -> ()
-  | t0 :: ts -> assert (forall (xs' : Dl.dlist ty) . exists (x : t0) (xs : Dl.dlist ts) .
-                         xs' == Dl.DCons t0 x ts xs);
-              introduce forall (x : t0) .
-                forall_dlist ts (partial_app_dlist t0 ts Type0 f x) <==>
-                (forall (xs : Dl.dlist ts) . f (Dl.DCons t0 x ts xs))
-              with forall_dlist_iff ts (partial_app_dlist t0 ts Type0 f x)
 
 let sl_all (ty : sl_tys_t) (f : sl_tys_v ty -> Type0)
   : Type0
   =
-   (forall (val_v : ty.val_t) . forall_dlist (ty.sel_t val_v) (fun sel_v -> f ({val_v; sel_v})))
+   (forall (val_v : ty.val_t) . Fl.forall_flist (ty.sel_t val_v) (fun sel_v -> f ({val_v; sel_v})))
 
 
 let sl_all_iff (ty : sl_tys_t) (f : sl_tys_v ty -> Type0)
@@ -829,29 +808,10 @@ let sl_all_iff (ty : sl_tys_t) (f : sl_tys_v ty -> Type0)
   =
     assert (forall (x : sl_tys_v ty) . x == {val_v = x.val_v; sel_v = x.sel_v})
 
-
-let rec exists_dlist (ty : Dl.ty_list) (f : Dl.dlist ty -> Type0)
-  : Tot Type0 (decreases ty)
-  = match ty with
-  | []     -> f Dl.DNil
-  | t0 :: ts -> (exists (x : t0) . exists_dlist ts (partial_app_dlist t0 ts Type0 f x))
-
-let rec exists_dlist_iff (ty : Dl.ty_list) (f : Dl.dlist ty -> Type0)
-  : Lemma (ensures exists_dlist ty f <==> (exists (xs : Dl.dlist ty) . f xs)) (decreases ty)
-          [SMTPat (exists_dlist ty f)]
-  = match ty with
-  | [] -> ()
-  | t0 :: ts -> assert (forall (xs' : Dl.dlist ty) . exists (x : t0) (xs : Dl.dlist ts) .
-                         xs' == Dl.DCons t0 x ts xs);
-              introduce forall (x : t0) .
-                exists_dlist ts (partial_app_dlist t0 ts Type0 f x) <==>
-                (exists (xs : Dl.dlist ts) . f (Dl.DCons t0 x ts xs))
-              with exists_dlist_iff ts (partial_app_dlist t0 ts Type0 f x)
-
 let sl_ex (ty : sl_tys_t) (f : sl_tys_v ty -> Type0)
   : Type0
   =
-   (exists (val_v : ty.val_t) . exists_dlist (ty.sel_t val_v) (fun sel_v -> f ({val_v; sel_v})))
+   (exists (val_v : ty.val_t) . Fl.exists_flist (ty.sel_t val_v) (fun sel_v -> f ({val_v; sel_v})))
 
 let sl_ex_iff (ty : sl_tys_t) (f : sl_tys_v ty -> Type0)
   : Lemma (sl_ex ty f  <==> (exists (x : sl_tys_v ty) . f x))
@@ -860,65 +820,42 @@ let sl_ex_iff (ty : sl_tys_t) (f : sl_tys_v ty -> Type0)
     assert (forall (x : sl_tys_v ty) . x == {val_v = x.val_v; sel_v = x.sel_v})
 
 
-// TODO? normalize Uv.(downgrade_val (raise_val _))
-noeq type raise_t (a : Type u#a) : Type u#(max a b) =
-  | Raise_val : (x : a) -> raise_t a
-
-let downgrade_val (#a : Type u#a) (y : raise_t u#a u#b a) : a
-  = let Raise_val x = y in x
-
-
-let rec arw_dlist (src : Dl.ty_list u#s) (dst : Type u#d)
-  : Tot (Type u#(max s d)) (decreases src)
-  = match src with
-  | [] -> raise_t dst
-  | t0 :: ts -> (t0 -> arw_dlist ts dst)
-
-let rec lam_dlist (src : Dl.ty_list u#s) (dst : Type u#d) (f : Dl.dlist src -> dst)
-  : Tot (arw_dlist src dst) (decreases src)
-  = match src with
-  | [] -> Raise_val (f Dl.DNil)
-  | t0 :: ts -> (fun (x : t0) -> lam_dlist ts dst (partial_app_dlist t0 ts dst f x))
-
-let rec app_dlist (#src : Dl.ty_list u#s) (#dst : Type u#d) (f : arw_dlist src dst) (x : Dl.dlist src)
-  : Tot dst (decreases src)
-  = match (|src, f, x|) <: (src : Dl.ty_list & arw_dlist src dst & Dl.dlist src) with
-  | (|[],      v, Dl.DNil|)           -> downgrade_val v
-  | (|t0 :: ts, f, Dl.DCons _ x _ xs|) -> app_dlist #ts #dst (f x) xs
-
-let rec app_lam_dlist (src : Dl.ty_list u#s) (dst : Type u#d) (f : Dl.dlist src -> dst) (x : Dl.dlist src)
-  : Lemma (ensures app_dlist (lam_dlist src dst f) x == f x)
-          (decreases src)
-          [SMTPat (app_dlist (lam_dlist src dst f) x)]
-  = match x with
-  | Dl.DNil -> ()
-  | Dl.DCons t0 x ts xs -> app_lam_dlist ts dst (partial_app_dlist t0 ts dst f x) xs
-
 let sl_arw (src : sl_tys_t u#a u#b) (dst : Type u#d) : Type =
-  (x : src.val_t) -> arw_dlist (src.sel_t x) dst
+  (x : src.val_t) -> Fl.arw_list (src.sel_t x) dst
 
-let sl_lam (src : sl_tys_t u#a u#b) (dst : Type u#d) (f : (x : src.val_t) -> (xs : Dl.dlist (src.sel_t x)) -> dst)
+let sl_lam (src : sl_tys_t u#a u#b) (dst : Type u#d) (f : (x : src.val_t) -> (xs : Fl.flist (src.sel_t x)) -> dst)
   : sl_arw src dst
-  = fun (x : src.val_t) -> lam_dlist (src.sel_t x) dst (f x)
+  = fun (x : src.val_t) -> Fl.lam_flist (src.sel_t x) dst (f x)
 
 let sl_app (#src : sl_tys_t u#a u#b) (#dst : Type u#d) (f : sl_arw src dst) (x : sl_tys_v src) : dst
-  = app_dlist (f x.val_v) x.sel_v
+  = Fl.app_flist (f x.val_v) x.sel_v
 
 let sl_app_lam (src : sl_tys_t u#a u#b) (dst : Type u#d)
-               (f : (x : src.val_t) -> (xs : Dl.dlist (src.sel_t x)) -> dst) (x : sl_tys_v src)
+               (f : (x : src.val_t) -> (xs : Fl.flist (src.sel_t x)) -> dst) (x : sl_tys_v src)
   : Lemma (ensures sl_app (sl_lam src dst f) x == f x.val_v x.sel_v)
           [SMTPat (sl_app (sl_lam src dst f) x)]
   = ()
 
+unfold
+let sl_uncurrify (#val_t : Type) (#sel_t : post_t val_t) (#dst : Type)
+                 (f : (v : val_t) -> (sls : Fl.flist (sel_t v)) -> dst)
+                 (x : sl_tys_v ({val_t; sel_t})) : dst
+  = f x.val_v x.sel_v
 
-let sl_tys : Fun.tys u#(max a b + 1) u#(max a (b + 1)) = {
+unfold
+let sl_tys' : Fun.tys' u#(max a b + 1) u#(max a (b + 1)) = {
   t = sl_tys_t u#a u#b;
   v = sl_tys_v u#a u#b;
   unit = {val_t = U.unit'; sel_t = (fun _ -> [])};
-  emp  = {val_v = U.Unit'; sel_v = Dl.DNil};
+  emp  = {val_v = U.Unit'; sel_v = Fl.nil};
   all  = sl_all;
   ex   = sl_ex;
 }
+
+let sl_tys : Fun.tys u#(max a b + 1) u#(max a (b + 1)) =
+  (**) introduce forall (x : sl_tys'.v sl_tys'.unit) . x == sl_tys'.emp
+  (**)   with Fl.nil_uniq x.sel_v;
+  sl_tys'
 
 
 let rec repr_Fun_of_Steel (#val_t : Type u#a) (#sel_t : post_t u#a u#b val_t) (t : prog_tree val_t sel_t)
@@ -926,14 +863,11 @@ let rec repr_Fun_of_Steel (#val_t : Type u#a) (#sel_t : post_t u#a u#b val_t) (t
         (decreases t)
   = match t with
   | Tspec a post req ens ->
-          Fun.Tspec ({val_t = a; sel_t = post}) req
-             (sl_app (sl_lam ({val_t = a; sel_t = post}) prop ens))
+          Fun.Tspec ({val_t = a; sel_t = post}) req (sl_uncurrify ens)
   | Tret a x post sl ->
-          Fun.Tret #sl_tys ({val_t = a; sel_t = post}) ({val_v = x; sel_v = sl})
+          Fun.Tret #sl_tys ({val_t = a; sel_t = post}) ({val_v = x; sel_v = Fl.flist_of_d sl})
   | Tbind a b itm post f g ->
-          Fun.Tbind _ _
-            (repr_Fun_of_Steel f)
-            (sl_app (sl_lam _ _ (fun v sl -> repr_Fun_of_Steel (g v sl))))
+          Fun.Tbind _ _ (repr_Fun_of_Steel f) (sl_uncurrify (fun x sls -> repr_Fun_of_Steel (g x sls)))
   | TbindP a b post wp f g ->
            Fun.TbindP a ({val_t = b; sel_t = post}) wp f (fun (x : a) -> repr_Fun_of_Steel (g x))
 
@@ -966,7 +900,7 @@ let rec repr_Fun_of_Steel_req #val_t #sel_t (t : prog_tree val_t sel_t)
           }
 
 and repr_Fun_of_Steel_ens #val_t #sel_t (t : prog_tree val_t sel_t)
-                          (val_v : val_t) (sel_v : Dl.dlist (sel_t val_v))
+                          (val_v : val_t) (sel_v : Fl.flist (sel_t val_v))
   : Lemma (ensures tree_ens t val_v sel_v <==> Fun.tree_ens (repr_Fun_of_Steel t) ({val_v; sel_v}))
           (decreases t)
   = match t with
@@ -974,7 +908,7 @@ and repr_Fun_of_Steel_ens #val_t #sel_t (t : prog_tree val_t sel_t)
           assert (tree_ens (Tspec a post req ens) val_v sel_v == ens val_v sel_v)
                by T.(trefl ());
           assert (Fun.tree_ens (repr_Fun_of_Steel (Tspec a post req ens)) ({val_v; sel_v})
-               == sl_app (sl_lam ({val_t = a; sel_t = post}) prop ens) ({val_v; sel_v}))
+               == sl_uncurrify ens ({val_v; sel_v}))
                by T.(trefl ())
   | Tret a x post sl -> ()
   | Tbind a b itm post f g ->
@@ -982,11 +916,14 @@ and repr_Fun_of_Steel_ens #val_t #sel_t (t : prog_tree val_t sel_t)
                == (exists (x : a) (sl1 : post_v itm x) . tree_ens f x sl1 /\ tree_ens (g x sl1) val_v sel_v) )
                by T.(trefl ());
           assert (Fun.tree_ens (repr_Fun_of_Steel (Tbind a b itm post f g)) ({val_v; sel_v})
-               == sl_tys.ex ({val_t=a; sel_t=itm}) (fun (x_sl1 : sl_tys_v ({val_t=a; sel_t=itm})) ->
+               == (let () = U.block_red in
+                   sl_tys.ex ({val_t=a; sel_t=itm}) (fun (x_sl1 : sl_tys_v ({val_t=a; sel_t=itm})) ->
                      Fun.tree_ens (repr_Fun_of_Steel f) x_sl1 /\
                      Fun.tree_ens
-                      (sl_app (sl_lam _ _ (fun v sl -> repr_Fun_of_Steel (g v sl))) x_sl1) ({val_v; sel_v})))
-               by T.(trefl ());
+                      (sl_uncurrify (fun x sls -> repr_Fun_of_Steel (g x sls)) x_sl1) ({val_v; sel_v}))))
+               by T.(norm [delta_only [`%repr_Fun_of_Steel; `%Fun.tree_ens]; zeta];
+                     norm [delta_only [`%U.block_red]; iota];
+                     trefl ());
           introduce forall (x : a) (sl1 : post_v itm x) .
                     (tree_ens f x sl1   <==> Fun.tree_ens (repr_Fun_of_Steel f) ({val_v=x; sel_v=sl1})) /\
                     (tree_ens (g x sl1) val_v sel_v <==> Fun.tree_ens (repr_Fun_of_Steel (g x sl1)) ({val_v; sel_v}))
