experiment/Experiment.Steel.Repr.Test.fst
@@ -5,6 +5,7 @@ module T    = FStar.Tactics
 module L    = FStar.List.Pure
 module Ll   = Learn.List
 module Dl   = Learn.DList
+module Fl   = Learn.FList
 module Perm = Learn.Permutation
 
 module M    = Experiment.Steel.Repr.M
@@ -28,20 +29,20 @@ let read_pre  (r : ref nat) : M.pre_t
 unfold
 let read_post (r : ref nat) : M.post_t nat
   = fun _ -> [vptr' r full_perm]
+unfold
 let read_req  (r : ref nat) : M.req_t (read_pre r)
   = fun sl0 -> True
+unfold
 let read_ens  (r : ref nat) : M.ens_t (read_pre r) nat (read_post r)
   = fun sl0 x sl1 ->
-    assert (L.length (M.vprop_list_sels_t (read_post r x)) == 1)
-      by T.(trefl ());
-    Dl.index sl1 0 == Dl.index sl0 0 /\ x == Dl.index sl0 0
+    sl1 0 == sl0 0 /\ x == sl0 0
 
 let steel_read0 (r : ref nat) () :
   Steel nat (M.vprop_of_list [vptr' r full_perm]) (fun _ -> M.vprop_of_list [vptr' r full_perm])
     (requires fun _ -> True)
     (ensures fun h0 x h1 -> let sl0 = M.rmem_sels [vptr' r full_perm] h0 in
                          let sl1 = M.rmem_sels [vptr' r full_perm] h1 in
-                         Dl.index sl1 0 == Dl.index sl0 0 /\ x == Dl.index sl0 0)
+                         sl1 0 == sl0 0 /\ x == sl0 0)
   =
     (**) change_equal_slprop (M.vprop_of_list [vptr' r full_perm]) (vptr r `star` emp);
     let x = read r in
@@ -148,7 +149,7 @@ let normal_shape_ST : list norm_step = [
 
 unfold
 let test0_SF (r : ref nat) (x_ini : nat) : SF.prog_tree _ _ =
-  SF.repr_Fun_of_ST (test0_ST r) (test0_shape_ST r) Dl.(DCons _ x_ini _ DNil)
+  SF.repr_Fun_of_ST (test0_ST r) (test0_shape_ST r) Fl.(cons x_ini nil)
 
 let normal_tree_SF : list norm_step = [
     delta_only [`%SF.repr_Fun_of_ST; `%SF.post_Fun_of_ST; `%SF.post_bij;
@@ -156,9 +157,12 @@ let normal_tree_SF : list norm_step = [
                 `%SF.Mkpost_bij_t'?.post'_n; `%SF.Mkpost_bij_t'?.post'_f; `%SF.Mkpost_bij_t'?.post'_g;
                 `%Ll.initi; `%L.index; `%L.hd; `%L.tl; `%L.tail; `%L.length;
                 `%SF.sel_ST_of_Fun; `%SF.post_src_of_shape; `%SF.sel_Fun_of_ST;
-                `%Dl.initi; `%Dl.splitAt_ty;
+                `%Fl.splitAt_ty; `%Fl.head; `%Fl.tail;
+                `%Fl.dlist_of_f; `%Dl.initi;
                 `%Mktuple2?._1;`%Mktuple2?._2;
-                `%Learn.Option.map];
+                `%Learn.Option.map;
+                `%Perm.perm_f_swap; `%Perm.perm_f_transpose; `%Perm.perm_f_of_pair;
+                `%Perm.mk_perm_f; `%Perm.id_n];
     delta_qualifier ["unfold"];
     delta_attr [`%U.__util_func__];
     iota; zeta; primops
@@ -171,16 +175,57 @@ let normal_tree_SF : list norm_step = [
               norm normal_tree_SF;
               qed ())*)
 
+unfold
+let test0_Fun (r : ref nat) (x_ini : nat) = 
+  SF.repr_Fun_of_Steel (test0_SF r x_ini)
+
+let normal_repr_Fun_of_Steel : list norm_step = [
+    delta_only [`%SF.repr_Fun_of_Steel];
+    delta_qualifier ["unfold"];
+    iota; zeta; primops
+  ]
+
+(*let _ = fun r x_ini ->
+    assert (print_util (test0_Fun r x_ini))
+        by T.(norm normal_tree_ST;
+              norm normal_shape_ST;
+              norm normal_tree_SF;
+              norm normal_repr_Fun_of_Steel;
+              qed ())*)
+
+unfold
+let test0_wp (r : ref nat) (x_ini : nat) =
+  Fun.tree_wp (test0_Fun r x_ini) (fun res -> res.val_v >= 0)
+
+let normal_spec_Fun : list norm_step = [
+    delta_only [`%Fun.tree_wp; `%Fl.partial_app_flist;
+                `%Fun.Mktys'?.all; `%SF.sl_tys; `%SF.sl_all; `%Fl.forall_flist;
+                `%Fl.cons; `%Fl.nil;
+                `%SF.Mksl_tys_t?.val_t; `%SF.Mksl_tys_t?.sel_t;
+                `%SF.Mksl_tys_v?.val_v; `%SF.Mksl_tys_v?.sel_v];
+    delta_qualifier ["unfold"];
+    iota; zeta; primops
+  ]
+
+(*let _ = fun r x_ini ->
+    assert (print_util (test0_wp r x_ini))
+        by T.(norm normal_tree_ST;
+              norm normal_shape_ST;
+              norm normal_tree_SF;
+              norm normal_repr_Fun_of_Steel;
+              norm normal_spec_Fun;
+              qed ())*)
+
 
 unfold
 let test1_ST : ST.prog_tree int [bool; int] (fun _ -> [bool; int])
   = ST.(
     b <-- Tframe _ _ _ [int] (
            Tspec bool [bool] (fun _ -> [bool])
-             (fun _ -> True) (fun sl0 b sl1 -> Dl.index sl1 0 = Dl.index sl0 0 /\ b = Dl.index sl0 0));
+             (fun _ -> True) (fun sl0 b sl1 -> sl1 0 = sl0 0 /\ b = sl0 0));
     Tequiv [bool; int] [int; bool] (Perm.perm_f_swap #2 0);;
     x <-- Tframe _ _ _ [bool] (Tspec int [int] (fun _ -> [int])
-           (fun _ -> True) (fun sl0 x sl1 -> Dl.index sl1 0 = Dl.index sl0 0 /\ x = Dl.index sl0 0));
+           (fun _ -> True) (fun sl0 x sl1 -> sl1 0 = sl0 0 /\ x = sl0 0));
     Tequiv [int; bool] [bool; int] (Perm.perm_f_swap #2 0);;
     Tret int (if b then x else 0) (fun _ -> [bool; int])
   )
@@ -210,7 +255,7 @@ let test1_shape_ST : ST.prog_shape test1_ST =
 
 unfold
 let test1_SF (b_ini : bool) (x_ini : int) : SF.prog_tree _ _ =
-  SF.repr_Fun_of_ST test1_ST test1_shape_ST Dl.(DCons _ b_ini _ (DCons _ x_ini _ DNil))
+  SF.repr_Fun_of_ST test1_ST test1_shape_ST Fl.(cons b_ini (cons x_ini nil))
 
 let norm_test_Fun : list norm_step
   = [delta_only [`%ST.bind; `%L.length; `%L.op_At; `%L.append];
@@ -226,7 +271,7 @@ let delta_only_repr_Fun_of_ST =
    `%SF.post_bij; `%SF.sel_ST_of_Fun; `%SF.sel_Fun_of_ST; `%SF.post_src_of_shape;
    `%ST.frame_post; `%ST.const_post]
 
-let norm_repr_Fun_of_ST : list norm_step
+let norm_repr_Fun_of_ST1 : list norm_step
   = [delta_only delta_only_repr_Fun_of_ST;
      delta_qualifier ["unfold"];
      delta_attr [`%U.__util_func__];
@@ -235,7 +280,7 @@ let norm_repr_Fun_of_ST : list norm_step
 (*let _ = fun b_ini x_ini ->
   assert (print_util (test1_SF b_ini x_ini))
     by T.(norm norm_test_Fun;
-          norm norm_repr_Fun_of_ST;
+          norm norm_repr_Fun_of_ST1;
           qed ())*)
 
 unfold
@@ -244,11 +289,11 @@ let test1_Fun (b_ini : bool) (x_ini : int) =
 
 let norm_repr_Fun_of_Steel : list norm_step
   = [delta_only (L.append delta_only_repr_Fun_of_ST
-                [`%SF.repr_Fun_of_Steel; `%SF.sl_lam; `%SF.lam_dlist; `%SF.partial_app_dlist;
+                [`%SF.repr_Fun_of_Steel; `%Fl.partial_app_flist;
                  `%SF.Mksl_tys_t?.val_t; `%SF.Mksl_tys_t?.sel_t;
-                 `%Dl.index; `%Dl.splitAt_ty; `%Mktuple2?._1; `%Mktuple2?._2;
-                 `%Dl.initi; `%L.length;
-                 
+                 `%Mktuple2?._1; `%Mktuple2?._2;
+                 `%L.length;
+
                  `%Perm.perm_f_swap; `%Perm.perm_f_transpose; `%Perm.perm_f_of_pair;
                  `%Perm.mk_perm_f]);
      delta_qualifier ["unfold"];
@@ -267,20 +312,19 @@ unfold
 let test2_SF : SF.prog_tree bool (fun _ -> [int]) = SF.(
   Tbind bool bool (fun _ -> [int; int]) (fun _ -> [int])
     (Tspec bool (fun _ -> [int; int]) True
-      (fun (b : bool) (xs : Dl.dlist [int; int]) ->
-         b ==> Dl.index xs 0 + Dl.index xs 1 >= 0))
-    (fun (b : bool) (xs : Dl.dlist [int; int]) ->
-      Tret bool (b && Dl.index xs 0 >= 0)
-              (fun _ -> [int]) Dl.(DCons int (index xs 0 + index xs 1) _ DNil)))
+      (fun (b : bool) (xs : Fl.flist [int; int]) ->
+         b ==> xs 0 + xs 1 >= 0))
+    (fun (b : bool) (xs : Fl.flist [int; int]) ->
+      Tret bool (b && xs 0 >= 0)
+              (fun _ -> [int]) Dl.(DCons _ (xs 0 + xs 1) _ DNil)))
 
 unfold
 let test2_Fun =
   SF.repr_Fun_of_Steel test2_SF
 
 let normal_tree_Fun : list norm_step = [
-    delta_only [`%SF.repr_Fun_of_Steel; `%SF.sl_lam; `%SF.lam_dlist; `%SF.partial_app_dlist;
-                `%SF.Mksl_tys_t?.val_t; `%SF.Mksl_tys_t?.sel_t;
-                `%Dl.index];
+    delta_only [`%SF.repr_Fun_of_Steel; `%Fl.partial_app_flist;
+                `%SF.Mksl_tys_t?.val_t; `%SF.Mksl_tys_t?.sel_t];
     delta_qualifier ["unfold"];
     iota; zeta; primops
   ]
@@ -294,16 +338,6 @@ let normal_tree_Fun : list norm_step = [
 unfold
 let test2_wp =
   Fun.tree_wp test2_Fun (fun x -> b2t x.val_v)
-
-let normal_spec_Fun : list norm_step = [
-    delta_only [`%Fun.tree_wp; `%SF.sl_app; `%SF.app_dlist; `%SF.partial_app_dlist;
-                `%Fun.Mktys'?.all; `%SF.sl_tys; `%SF.sl_all; `%SF.forall_dlist;
-                `%SF.Mksl_tys_t?.val_t; `%SF.Mksl_tys_t?.sel_t;
-                `%SF.Mksl_tys_v?.val_v; `%SF.Mksl_tys_v?.sel_v;
-                `%SF.downgrade_val];
-    delta_qualifier ["unfold"];
-    iota; zeta; primops
-  ]
 
 (*#push-options "--print_full_names"
 let _ =
